introduce UniqueKeyInFlight predicate

messageInvariantPrototypes/shardedKvBatched/hosts.dfy
@@ -124,15 +124,18 @@ module Host {
     && (forall k | k in msg.vks :: v.HasKey(k))
     && v' == v.(
       myKeys := (map k | k in v.myKeys
-          :: if k in msg.vks && v.myKeys[k].version < msg.vks[k] // in-flight definition
+          :: if UniqueKeyInFlight(c, v, k, msg)
               then Entry(true, msg.vks[k])
               else Entry(false, v.myKeys[k].version))
     )
   }
 
-  // ghost predicate UniqueKeyInFlight(c: Constants, v: Variables, key: UniqueKey, msg: Message) {
-
-  // }
+  // Uniqueness in-flight definition
+  ghost predicate UniqueKeyInFlight(c: Constants, v: Variables, key: UniqueKey, msg: Message) {
+    && key in v.myKeys
+    && key in msg.vks 
+    && v.myKeys[key].version < msg.vks[key]
+  }
 
   ghost predicate Next(c: Constants, v: Variables, v': Variables, msgOps: MessageOps)
   {
